work on iterator/generator

PivotBetree/BucketGenerator.i.dfy
@@ -1,12 +1,55 @@
-include "BucketsLib.i.dfy"
+include "BucketIterator.i.dfy"
+//
+// A mathematical description of bucket generators.
+// It's like an iterator, but it doesn't directly refer to an actual bucket.
+// The bucket may be implicit.
+//
 
 module BucketGenerator {
   import opened Options
+  import opened Maps
   import opened BucketsLib
   import opened PivotsLib
   import opened ValueMessage
   import opened Sequences
   import opened BucketIterator
-t
-  
+
+  datatype Generator =
+    | BasicGenerator(
+        // "Internals":
+        bucket: Bucket,
+        it: Iterator,
+
+        // Bucket that the generator represents
+        ghost remains: Bucket
+      )
+
+  protected predicate WF(g: Generator)
+  {
+    && WFIter(g.bucket, g.it)
+    && (g.it.next.Done? ==> g.remains == map[])
+    && (g.it.next.Next? ==> Keyspace.minimumOpt(g.remains.Keys) == Some(g.it.next.key))
+  }
+
+  // Generator operations:
+
+  function {:opaque} GenTop(g: Generator) : (next : IteratorOutput)
+  requires WF(g)
+  ensures next.Done? ==> g.remains == map[]
+  ensures next.Next? ==> Keyspace.minimumOpt(g.remains.Keys) == Some(next.key)
+  {
+    g.it.next
+  }
+
+  function {:opaque} GenPop(g: Generator) : (g' : Generator)
+  requires WF(g)
+  requires GenTop(g).Next?
+  ensures WF(g')
+  ensures g'.remains == MapRemove1(g.remains, GenTop(g).key)
+  {
+    BasicGenerator(
+        g.bucket,
+        IterInc(g.bucket, g.it),
+        MapRemove1(g.remains, GenTop(g).key))
+  }
 }
